theories/iris.v
@@ -237,13 +237,13 @@ Proof.
     apply: Hreds. }
   (* there must be a better way *)
   { move => cl _ _ _ _ es _ _ _ _ _ _ _ _ _ _ _ _ _ _ _ _ H.
-    assert (seq.size (es ++ [Callcl cl]) = @seq.size administrative_instruction []) as Hx; first by f_equal.
+    assert (seq.size (es ++ [Invoke cl]) = @seq.size administrative_instruction []) as Hx; first by f_equal.
     by apply: foo3. }
   { move => cl f t1s t2s es ves vcs _ _ _ _ _ _ _ _ _ _ _ _ H.
-    assert (seq.size (es ++ [Callcl cl]) = @seq.size administrative_instruction []) as Hx; first by f_equal.
+    assert (seq.size (es ++ [Invoke cl]) = @seq.size administrative_instruction []) as Hx; first by f_equal.
     by apply: foo3. }
   { move => cl _ _ _ es _ _ _ _ _ _ _ _ _ _ _ H.
-    assert (seq.size (es ++ [Callcl cl]) = @seq.size administrative_instruction []) as Hx; first by f_equal.
+    assert (seq.size (es ++ [Invoke cl]) = @seq.size administrative_instruction []) as Hx; first by f_equal.
       by apply: foo3. }
   { move => s vs es les i s' vs' le's les' k lh Hred Hes Hfill Hfill' Hles.
     by apply: (foo5 Hfill). }
